\rhead{27 October 2017}

\begin{Lem}
Suppose $x,y,m,n \in \Z$ with $m \not \equiv n \mod p$.
$x+y\zeta^n$ and $x+y\zeta^m$ are relatively prime $\iff$ ($x$ and $y$ are relatively prime) and ($x+y$ not divisible by $p$)
\end{Lem}

\begin{proof}
\glqq $\Rightarrow$\grqq: \begin{itemize}
\item $d|x$ and $d|y \Rightarrow d|x+\zeta^ny$ and $d| x+\zeta^ny$ \Lightning
\item \glqq $p| x+y$\grqq\ Recall: $p= \varepsilon (1-\zeta)^{p-1}$ with $\varepsilon \in O^\times\\
\Rightarrow x+\zeta^my = \underbrace{x+y}_{\text{divisible by } p} +y\cdot\underbrace{(\zeta^m-1)}_{(\zeta-1)(1+\zeta+\zeta^2\dots + \zeta^{m-1})} \equiv 0 \mod 1-\zeta$\\
same way $x+\zeta^ny \equiv 0 \mod 1- \zeta$ \Lightning
\end{itemize}
\glqq $\Leftarrow$\grqq: \underline{Idea:} show: $\exists \alpha_0, \beta_0 \in \O$ with:
\[1= \alpha_0(x+\zeta^m y) + \beta (x+ \zeta^ny)\]
Consider: $A:= \{\alpha (x+\zeta^my)+\beta(x+\zeta^ny) \ | \ \alpha,\beta \in \O \}$\\
$A$ is an ideal in $\O$. We have:
\begin{enumerate}
\item $(x+\zeta^m y) - (x+\zeta^n y) = \zeta^m(1-\zeta^{n-m})y= \underbrace{\zeta^n\varepsilon_{n-m}}_{\in \O^\times} (1 - \zeta)y \Rightarrow (1 - \zeta)y \in A$
\item $\zeta^n (x+ \zeta^my) - \zeta^m(x+\zeta^ny)=(\zeta^n-\zeta^m)x= \zeta^n\cdot(1-\zeta^{n-m})x=\underbrace{\zeta^n \varepsilon_{m-n}}_{\in \O^\times} \cdot (1- \zeta)x \Rightarrow (1- \zeta) x \in A$.
\item $\gcd(x,y)=1 \Rightarrow \exists \ a,b \in \Z$ with $1=ax+by \Rightarrow (1-\zeta)xa +(1-\zeta)yb = 1-\zeta \stackrel{1.\& 2.}{\Rightarrow} 1- \zeta \in A$
\item $x+y = \underbrace{x+ \zeta^ny}_{\in A} + \underbrace{(1- \zeta^n)y}_{\in A} \in A$
\item $\gcd(p,x+y)=1 \Rightarrow \exists \bar{a}, \bar{b} \in \Z: 1= \underbrace{\bar{a}p}_{\in A}+\bar{b}\underbrace{(x+y)}_{\in A} \in A$.\\
$\Rightarrow$ Hence $x+\zeta^ny$ and $x+ \zeta^my$ are coprime.
\end{enumerate}
\end{proof}

\begin{Bem}
Suppose $\alpha = a_0 + a_1 \zeta + \dots + a_{p-1}\zeta^{p-1} \in \O$ with $a_i \in \Z$ and at least one $a_j =0$.\\
If $n \in \Z$ with $n$ divides $\alpha$ in $\O$, then $n$ divides all $a_i$
\end{Bem}
\begin{proof}
Recall from 2.2 (preview): $1, \zeta, \zeta^2, \dots, \zeta^{p-2}$ is a basis of $\O$.\\
Furthermore: $1+\zeta+\dots+\zeta^{p-1}=0$\\
$\Rightarrow \{1, \zeta, \dots, \zeta^{p-1}\} \setminus \{\zeta^j\}$ is a basis $\Rightarrow$ claim.
\end{proof}

\section{First case of Fermat in case of $\Z[\zeta]$ is a UFD (unique factorization domain)}
Reference: BOREVICH + SHAFEREVIC + WASHINGTON Chapter 1\\
As before: $p$ odd prime, $\zeta= e^{\frac{2 \pi i}{p}} p$-th root of unity.

\begin{Satz}
Suppose that $\Z[\zeta]$ is a UFD, then $x^p+y^p=z^p$ has no non-trivial solutions $(x,y,z)$, such that neither $x,y$ nor $z$ is divisible by $p$.
\end{Satz}


\begin{Satz}[$p=3$]
Suppose $x,y,z \in \Z$ with $x^3+y^3=z^3 \mod 9 \Rightarrow 3$ divides $x,y$ or $z$.
\end{Satz}
\begin{proof}
Recall: Little Fermat's theorem $x^p \equiv x, y^p \equiv y, z^p\equiv z \mod p$.
\begin{align*}
x^3+y^3=z^3 \mod 3 \Rightarrow x+y \equiv z \mod 3\\
\Rightarrow z=x+y+3u \text{ with } u \in \Z\\
\Rightarrow \underline{x^3+y^3} \equiv (x+y+3u)^3 \equiv \underline{x^3+y^3}+3xy^2+3x^2y \mod 9\\
\Rightarrow 0 \equiv xy^3+x^2y \equiv xy(x+y) \equiv xyz \mod 3\\
\Rightarrow x,y \text{ or } z \text{ is divisible by } 3
\end{align*}
\end{proof}

\begin{Lem}
Let $p \geq 5$. Suppose $x,y,z \in \Z$ with $x^p+y^p=z^p$. If $x\equiv y \equiv -z \mod p$, then $p | z$.
\end{Lem}
\begin{proof}
$z \equiv z^p = x^p+y^p \equiv -2z^p \equiv -2z \mod p \Rightarrow 3z \equiv 0 \mod p \stackrel{p \neq 3}{\Longrightarrow} p | z$.
\end{proof}

\begin{Bem}
It follows from Lemma 3.2 that in the first case of Fermat we may assume for $p \geq 5$ that $x \not\equiv y \mod p$ because we can replace $x^p + y^p = z^p $ by $x^p+(-z)^p=(-y)^p$ and $x \not\equiv -z \mod p$.
\end{Bem}

\begin{proof}[of Thm. 1]
$p=3 \Rightarrow $ claim follows from Prop 3.1.\\
Now: $p \geq 5$. Suppose $x,y,z \in \Z$ with $p$ divides neither $x,y$ nor $z$, $x,y,z$ are pairwise coprime and $x \not\equiv y \mod p$. Suppose $z^p = x^p +y^p=(x+y)(x+\zeta y)\dots (x+\zeta^{p-1}y)$.\\
Apply Lemma 2.11:
\begin{itemize}
\item $\gcd(x,y)=1$ \checkmark
\item Little Fermat $\Rightarrow x+y \equiv x^p+y^p\equiv z^p \not \equiv 0 \mod p$
\end{itemize}
$\stackrel{2.11}{\Longrightarrow} x+y, x+\zeta y, \dots, x+\zeta^{p-1}y$ are pairwise coprime.\\
$\stackrel{\Z[\zeta] \text{ UFD}}{\Longrightarrow}$ \glqq $x+\zeta^i y$ have to be $p$-power\grqq \ More precisely: $x+\zeta y = \varepsilon \alpha^p$ with $\varepsilon \in \O^\times, \alpha \in \O$, since they are coprime factors of a $p$-th power.
\begin{enumerate}
\item Cor. 2.10 $\Rightarrow \varepsilon = r \zeta^s$ with $r \in \R, s \in \Z$
\item Example 2.8. iii) $\Rightarrow \exists a \in \Z$ with $\alpha^p \equiv a \mod p$.
\begin{align*}
x + \zeta y = r \zeta^s \alpha^p \equiv r \zeta^s a \mod p\\
x+ \zeta^{-1} y = \overline{x+ \zeta y} \equiv r \zeta^{-s}a \mod p\\
\Rightarrow \zeta^{-s}(x+\zeta y) \equiv ra \equiv \zeta^s(x+\zeta^{-1}y) \mod p\\
\Rightarrow \underbrace{x+\zeta y - \zeta^{2s}x- \zeta^{2s-1}y}_{=x\cdot 1 + y \zeta -x \zeta^{2s} - y \zeta^{2s-1}} \equiv 0 \mod p\\
\end{align*}
Idea: Use Rem. 2.12\\
\underline{Case 1:} $1, \zeta, \zeta^{2s-1}, \zeta^{2s}$ are distinct $\stackrel{p \geq 5, \text{ Rem 2.12}}{\Longrightarrow} p | x$ and $p | y$.  Contradiction to first case.
\end{enumerate}
\end{proof}